

The formulae were reverse engineered from the work of *The Weil Pairing on Elliptic Curves and Its Cryptographic Applications, Appendix D*, 2011. A.E. Aftuk.

Operations in  $\mathbb{F}_{p^2}$ , distortion parameter  $\beta$ , curve  $E : y^2 = x^3 + 1$ .

**Multiplication of scalars**  $\text{mul}_\beta(x, y)$ :

$$\begin{aligned}
 a &\leftarrow x \bmod \beta \\
 b &\leftarrow (x \bmod \beta^2) - a \\
 c &\leftarrow y \bmod \beta \\
 d &\leftarrow (y \bmod \beta^2) - c \\
 \mathbf{return} & (ac - bd) + \beta(ad + bc - bd) \bmod p
 \end{aligned} \tag{1}$$

**Power of scalars**  $\text{pow}_\beta(x, y)$ :

$$\begin{aligned}
 r &\leftarrow 1 \\
 \mathbf{while} & x > 0 \\
 | & \mathbf{if} x = 1 \bmod 2 \\
 | & | r \leftarrow \text{mul}_\beta(r, y) \\
 | & y \leftarrow \text{mul}_\beta(y, y) \\
 | & x \leftarrow \left\lfloor \frac{x}{2} \right\rfloor \\
 \mathbf{return} & r
 \end{aligned} \tag{2}$$

**Inverse of scalar**  $\text{inv}_\beta(x)$ :

$$\begin{aligned}
 a &\leftarrow x \bmod \beta \\
 b &\leftarrow (x \bmod \beta^2) - a \\
 \mathbf{return} & \frac{a - b}{a^2 - ab + b^2} - \beta \frac{b}{a^2 - ab + b^2} \bmod p
 \end{aligned} \tag{3}$$

**Sum of points on E**  $\text{sum}_E(P, Q)$ :

```

if  $P = "O"$  and  $Q = "O"$ 
  | return  $"O"$ 
if  $P = "O"$ 
  | return  $Q$ 
and  $Q = "O"$ 
  | return  $P$ 
 $x_1, y_1 \leftarrow P$ 
 $x_2, y_2 \leftarrow Q$ 
if  $(x_1 \bmod p) = (x_2 \bmod p)$  and  $(y_1 \bmod p) = (-y_2 \bmod p)$ 
  | return  $"O"$ 
if  $(x_1 \bmod p) = (x_2 \bmod p)$ 
  |  $\lambda \leftarrow \frac{3x_1^2}{2y_1} \bmod \beta^2 + \beta + 1$ 
else
  |  $\lambda \leftarrow \frac{y_1 - y_2}{x_1 - x_2} \bmod \beta^2 + \beta + 1$ 
 $x_3 \leftarrow \lambda^2 - x_1 - x_2 \bmod \beta^2 + \beta + 1$ 
 $x_3 \leftarrow \lambda(x_3 - x_1) + y_1 \bmod \beta^2 + \beta + 1$ 
return  $\{x_3, -y_3 \bmod p\}$ 

```

(4)

**Calculate  $x \times P$  using double-and-add method**  $\text{dadd}_E(x, P)$ :

```

 $R \leftarrow "O"$ 
while  $x > 0$ 
  | if  $x = 1 \bmod 2$ 
  |   |  $r \leftarrow \text{sum}_E(R, P)$ 
  |   |  $P \leftarrow \text{sum}_E(P, P)$ 
  |   |  $x \leftarrow \lfloor \frac{x}{2} \rfloor$ 
return  $r$ 

```

(5)

$H(P, Q)$ :

```

x1, y1 ← P
x2, y2 ← Q
if (x1 mod p) = (x2 mod p) and (y1 mod p) = (-y2 mod p)
  | return x - x1 mod β2 + β + 1
if (x1 mod p) = (x2 mod p) and (y1 mod p) = (y2 mod p)
  | λ ←  $\frac{3x1^2}{2y1}$  mod β2 + β + 1
  | return  $\frac{y - y1 - \lambda(x - x1)}{x + x1 + x2 - \lambda^2}$  mod β2 + β + 1
if (x1 mod p) ≠ (x2 mod p)
  | λ ←  $\frac{y2 - y1}{x2 - x1}$  mod β2 + β + 1
  | return  $\frac{y - y1 - \lambda(x - x1)}{x + x1 + x2 - \lambda^2}$  mod β2 + β + 1

```

Perform the Miller calculation  $\text{miller}_E(m, P, R)$ :

```

f ← 1
T ← P
mlist ← reversed(as_binary(m))
for i in reversed(range(length(mlist)))
  | f ← f2H(T, T) mod β2 + β + 1
  | f ← eval(f, x = R[0], y = R[1]) mod β2 + β + 1
  | T ← sumE(T, T)
  | if mlist[i] = 1
    | f ← fH(T, P) mod β2 + β + 1
    | T ← sumE(T, P)
  | f ← eval(f, x = R[0], y = R[1]) mod β2 + β + 1
return f

```

Create a weil pairing  $\text{pairing}_E(m, P, Q, S)$ :

$$\begin{aligned} nS &\leftarrow \{S[0], -S[1]\} \bmod \beta^2 + \beta + 1 \\ A &\leftarrow \text{miller}_E(m, P, \text{sum}_E(Q, S)) \\ B &\leftarrow \text{miller}_E(m, P, S) \\ C &\leftarrow \text{miller}_E(m, Q, \text{sum}_E(P, nS)) \\ D &\leftarrow \text{miller}_E(m, Q, nS) \\ WP &\leftarrow \frac{AD}{BC} \bmod \beta^2 + \beta + 1 \\ \text{return } &\text{numerator}(WP) \times \text{inv}_\beta(\text{denominator}(WP)) \bmod \beta^2 + \beta + 1 \end{aligned} \tag{8}$$